some changes to bigstep for proof

project/Big_Small_Eq.v
@@ -1,4 +1,4 @@
-(* Add LoadPath "C:\\Users\\ument\\School\\cs522\\cs522_project\\project". *)
+Add LoadPath "C:\\Users\\ument\\School\\cs522\\cs522_project\\project".
 Add LoadPath "/Users/brandomiranda/home_simulation_research/cs522_project/project".
 Require Import Imp_Syntax.
 Require Import Imp_Big_Step.
@@ -6,13 +6,25 @@ Require Import Imp_Small_Step.
 Require Import Coq.Strings.String.
 
 Definition State := string -> (option nat).
-
+Definition ConfigEquivR (C1 C2 : SmallConfig) :=
+  exists N : nat, NSmallSteps N C1 C2.
+  
 Theorem Big_Small_Equiv : forall (P : Program) (S : State),
-  (BigStepR (B_PgmConf P) (B_StateConf S)) <-> (SmallStepR (S_PgmConf P) (S_BlkConf EmptyBlk S)).
+  (BigStepR (B_PgmConf P) (B_StateConf S)) <-> (ConfigEquivR (S_PgmConf P) (S_BlkConf EmptyBlk S)).
   intros.
   split.
   induction P.
   intros.
+  unfold ConfigEquivR. refine (ex_intro _ _ _) . admit. (*
+  refine (Succ _ _ _ _) .
+  intros.
   generalize dependent s.
-  induction s ; intros.
+  induction s ; intros ; unfold ConfigEquivR . *)
+  generalize dependent P.
+  induction P .
+  intros.
+  apply BigStep_Pgm.
+  unfold ConfigEquivR in H.
+  induction s.
+  refine (BigStep_Assign _ _ _ _).
 Admitted.
